CertiGC/GraphGC.v
@@ -1,0 +1,159 @@
+Require Import Coq.ZArith.ZArith.
+Require Import Coq.Lists.List.
+Require Import RamifyCoq.lib.Coqlib.
+Require Import RamifyCoq.lib.EquivDec_ext.
+
+Require Import RamifyCoq.graph.graph_model.
+Require Import RamifyCoq.msl_application.Graph.
+
+Require Import RamifyCoq.graph.reachable_computable.
+Require Import RamifyCoq.graph.MathGraph.
+Require Import RamifyCoq.graph.FiniteGraph.
+
+Class pPointwiseGraph_GC: Type :=
+  {
+    val: Type;
+    null: val;
+    SGBA: PointwiseGraphBasicAssum val (val * nat)
+  }.
+
+Existing Instance SGBA.
+
+Definition is_null_SGBA {pSGG: pPointwiseGraph_GC} : DecidablePred val :=
+  (existT (fun P => forall a, {P a} + {~ P a})
+          (fun x => x = null) (fun x => SGBA_VE x null)).
+
+Section GC_Graph.
+
+  Context {pPG_GC: pPointwiseGraph_GC}.
+
+  Inductive raw_field : Type :=
+  | raw_data : val -> raw_field
+  | raw_pointer : raw_field.
+  
+  Record raw_vertex_block : Type :=
+    {
+      raw_mark: bool;
+      raw_fields: list raw_field;
+      raw_color: Z;
+      raw_tag: Z;
+    }.
+
+  Record space: Type :=
+    { 
+      start: val;
+      used_space: nat;
+      rest_space: nat;
+    }.
+
+  Record heap: Type :=
+    {
+      spaces: list space;
+    }.
+
+  Definition LGraph := LabeledGraph val (val * nat) raw_vertex_block unit heap.
+
+  Fixpoint get_edges' (lf: list raw_field) (v: val) (n: nat) : list (val * nat) :=
+    match lf with
+    | nil => nil
+    | cons x lf' => match x with
+                    | raw_data _ => get_edges' lf' v (n + 1)
+                    | raw_pointer => (v, n) :: get_edges' lf' v (n + 1)
+                    end
+    end.
+
+  Definition get_edges (g: LGraph) (v: val) :=
+    get_edges' (raw_fields (vlabel g v)) v O.
+
+  Lemma get_edges'_range: forall v n l m,
+      In (v, n) (get_edges' l v m) -> m <= n < m + length l.
+  Proof.
+    intros v n l. revert v n. induction l; simpl; intros. 1: exfalso; auto.
+    specialize (IHl v n (m + 1)). destruct a. 1: apply IHl in H; omega.
+    simpl in H. destruct H. 1: inversion H; omega. apply IHl in H. omega.
+  Qed.
+
+  Lemma get_edges'_nth: forall n l a m v,
+      n < length l -> nth n l a = raw_pointer <-> In (v, n + m) (get_edges' l v m).
+  Proof.
+    induction n.
+    - induction l; simpl; intros. 1: inversion H. destruct a.
+      + split; intros. inversion H0. apply get_edges'_range in H0. exfalso; omega.
+      + simpl. intuition.
+    - destruct l; simpl; intros. 1: inversion H. assert (n < length l) by omega.
+      specialize (IHn l a (m + 1) v H0).
+      replace (n + (m + 1)) with (S (n + m)) in IHn by omega. rewrite IHn.
+      destruct r; intuition. simpl in H3. destruct H3; auto. inversion H3. omega.
+  Qed.
+
+  Local Coercion pg_lg: LabeledGraph >-> PreGraph.
+
+  Class SoundGCGraph (g: LGraph) :=
+    {
+      fin: FiniteGraph g;
+      field_decided_edges: forall v e,
+          vvalid g v -> (src g e = v /\ evalid g e <-> In e (get_edges g v));
+      (* Other constraints would be added later *)
+    }.
+
+  Definition Graph :=
+    GeneralGraph val (val * nat) raw_vertex_block unit heap (fun g => SoundGCGraph g).
+
+  Record vertex_block :=
+    {
+      v_mark: bool;
+      v_fields: list val;
+      v_color: Z;
+      v_tag: Z;
+    }.
+
+  Definition SGraph := PointwiseGraph val (val * nat) vertex_block unit.
+
+  Fixpoint make_fields' (g: LGraph) (lf : list raw_field)
+           (v : val) (n : nat) : list val :=
+    match lf with
+    | nil => nil
+    | cons x lf' => match x with
+                    | raw_data d => d :: make_fields' g lf' v (n + 1)
+                    | raw_pointer => dst g (v, n) :: make_fields' g lf' v (n+1)
+                  end
+    end.
+
+  Definition make_fields (g: LGraph) (v: val) :=
+    make_fields' g (raw_fields (vlabel g v)) v O.
+
+  Definition gen_vertex_gamma (g: LGraph) (v: val): vertex_block :=
+    Build_vertex_block (raw_mark (vlabel g v))
+                       (make_fields g v)
+                       (raw_color (vlabel g v))
+                       (raw_tag (vlabel g v)).
+
+  Instance SGC_GC: PointwiseGraphConstructor
+                     val (val * nat) raw_vertex_block unit heap vertex_block unit.
+  Proof.
+    constructor. exact gen_vertex_gamma. exact (fun _ _ => tt).
+  Defined.
+
+  Instance LSGC_GC: Local_PointwiseGraphConstructor val (val * nat) raw_vertex_block unit heap vertex_block unit.
+  Proof.
+    refine (Build_Local_PointwiseGraphConstructor
+              _ _ _ _ _ _ _ SGBA SGC_GC
+              (fun G v => forall e, In e (get_edges G v) -> evalid G e /\ src G e = v)
+              _ (fun G e => True) _); trivial.
+    simpl. intros. unfold gen_vertex_gamma. rewrite H1. f_equal.
+    unfold make_fields. rewrite H1. remember (raw_fields (vlabel G2 x)) as l.
+    clear Heql. remember 0 as n. clear Heqn. revert n. induction l; intros; simpl.
+    1: reflexivity. destruct a. 1: f_equal; rewrite IHl; reflexivity.
+    rewrite IHl. f_equal.
+  Abort.
+
+  Class sPointwiseGraph_GraphGC: Type :=
+    {
+      pred: Type;
+      PGP: PointwiseGraphPred val (val * nat) vertex_block unit pred;
+      PGA: PointwiseGraphAssum PGP;
+      PGAvs: PointwiseGraphAssum_vs PGP;
+      PGAvn: PointwiseGraphAssum_vn PGP null
+    }.
+
+End GC_Graph.
